Start to fix the transcripts

fstar/new/MLS.TreeDEM.Message.Framing.fst
@@ -3,38 +3,16 @@ module MLS.TreeDEM.Message.Framing
 open Lib.IntTypes
 open MLS.TreeDEM.Keys
 open MLS.TreeDEM.Message.Content
+open MLS.TreeDEM.Message.Transcript
 open Lib.ByteSequence
 open MLS.Crypto
 open MLS.NetworkTypes
+open MLS.TreeDEM.Message.Types
 open MLS.NetworkBinder
 open MLS.Parser
 open MLS.Result
 
 module NT = MLS.NetworkTypes
-
-type sender_type =
-  | ST_member
-  | ST_preconfigured
-  | ST_new_member
-
-type sender = {
-  sender_type: sender_type;
-  sender_id: nat;
-}
-
-noeq type message = {
-  group_id: bytes;
-  epoch: nat;
-  sender: sender;
-  authenticated_data: bytes;
-  content_type: message_content_type;
-  message_content: message_content content_type;
-}
-
-noeq type message_auth = {
-  signature: bytes;
-  confirmation_tag: option bytes;
-}
 
 noeq type message_plaintext = {
   group_id: bytes;
@@ -71,57 +49,6 @@ noeq type encrypted_sender_data_content = {
 }
 
 (*** From/to network ***)
-
-val network_to_sender_type: sender_type_nt -> result sender_type
-let network_to_sender_type s =
-  match s with
-  | NT.ST_member -> return ST_member
-  | NT.ST_preconfigured -> return ST_preconfigured
-  | NT.ST_new_member -> return ST_new_member
-  | _ -> error "network_to_sender_type: invalid sender type"
-
-val sender_type_to_network: sender_type -> sender_type_nt
-let sender_type_to_network s =
-  match s with
-  | ST_member -> NT.ST_member
-  | ST_preconfigured -> NT.ST_preconfigured
-  | ST_new_member -> NT.ST_new_member
-
-val network_to_sender: sender_nt -> result sender
-let network_to_sender s =
-  sender_type <-- network_to_sender_type s.sender_type;
-  return ({
-    sender_type = sender_type;
-    sender_id = Lib.IntTypes.v s.sender;
-  })
-
-val sender_to_network: sender -> result sender_nt
-let sender_to_network s =
-  if not (s.sender_id < pow2 32) then (
-    internal_failure "network_to_sender: sender_id too big"
-  ) else (
-    return ({
-      sender_type = sender_type_to_network s.sender_type;
-      sender = u32 s.sender_id;
-    } <: sender_nt)
-  )
-
-val opt_tag_to_opt_bytes: option_nt mac_nt -> result (option bytes)
-let opt_tag_to_opt_bytes mac =
-  optmac <-- network_to_option mac;
-  return (
-    match optmac with
-    | None -> (None <: option bytes)
-    | Some m -> Some (m.mac_value)
-  )
-
-val opt_bytes_to_opt_tag: option bytes -> result (option_nt mac_nt)
-let opt_bytes_to_opt_tag mac =
-  optmac <-- (match mac with
-    | None -> (return None)
-    | Some m -> if Seq.length m < 256 then return (Some ({mac_value = m})) else internal_failure "opt_bytes_to_opt_tag: mac too long"
-  );
-  return (option_to_network optmac)
 
 val network_to_message_plaintext: mls_plaintext_nt -> result message_plaintext
 let network_to_message_plaintext pt =
@@ -327,12 +254,20 @@ let compute_message_membership_tag cs membership_key msg auth group_context =
   hmac_hmac cs membership_key serialized_bytes
 
 val message_compute_auth: cs:ciphersuite -> message -> sign_private_key cs -> randomness (sign_nonce_length cs) -> group_context:bytes -> bytes -> bytes -> result message_auth
-let message_compute_auth cs msg sk rand group_context confirmation_key confirmed_transcript_hash =
+let message_compute_auth cs msg sk rand group_context confirmation_key interim_transcript_hash =
   signature <-- compute_message_signature cs sk rand msg group_context;
-  confirmation_tag <-- compute_message_confirmation_tag cs confirmation_key confirmed_transcript_hash;
+  confirmation_tag <-- (
+    if msg.content_type = Content.CT_commit then (
+      confirmed_transcript_hash <-- compute_confirmed_transcript_hash cs msg signature interim_transcript_hash;
+      confirmation_tag <-- compute_message_confirmation_tag cs confirmation_key confirmed_transcript_hash;
+      return (Some confirmation_tag <: option bytes)
+    ) else (
+      return None
+    )
+  );
   return ({
     signature = signature;
-    confirmation_tag = Some (confirmation_tag);
+    confirmation_tag = confirmation_tag;
   } <: message_auth)
 
 (*** From/to plaintext ***)
