fstar/new/MLS.TreeDEM.Message.Types.fst
@@ -1,0 +1,85 @@
+module MLS.TreeDEM.Message.Types
+
+open Lib.ByteSequence
+open Lib.IntTypes
+open MLS.NetworkTypes
+open MLS.NetworkBinder
+open MLS.TreeDEM.Message.Content
+open MLS.Result
+
+module NT = MLS.NetworkTypes
+
+type sender_type =
+  | ST_member
+  | ST_preconfigured
+  | ST_new_member
+
+type sender = {
+  sender_type: sender_type;
+  sender_id: nat;
+}
+
+noeq type message = {
+  group_id: bytes;
+  epoch: nat;
+  sender: sender;
+  authenticated_data: bytes;
+  content_type: message_content_type;
+  message_content: message_content content_type;
+}
+
+noeq type message_auth = {
+  signature: bytes;
+  confirmation_tag: option bytes;
+}
+
+val network_to_sender_type: sender_type_nt -> result sender_type
+let network_to_sender_type s =
+  match s with
+  | NT.ST_member -> return ST_member
+  | NT.ST_preconfigured -> return ST_preconfigured
+  | NT.ST_new_member -> return ST_new_member
+  | _ -> error "network_to_sender_type: invalid sender type"
+
+val sender_type_to_network: sender_type -> sender_type_nt
+let sender_type_to_network s =
+  match s with
+  | ST_member -> NT.ST_member
+  | ST_preconfigured -> NT.ST_preconfigured
+  | ST_new_member -> NT.ST_new_member
+
+val network_to_sender: sender_nt -> result sender
+let network_to_sender s =
+  sender_type <-- network_to_sender_type s.sender_type;
+  return ({
+    sender_type = sender_type;
+    sender_id = Lib.IntTypes.v s.sender;
+  })
+
+val sender_to_network: sender -> result sender_nt
+let sender_to_network s =
+  if not (s.sender_id < pow2 32) then (
+    internal_failure "network_to_sender: sender_id too big"
+  ) else (
+    return ({
+      sender_type = sender_type_to_network s.sender_type;
+      sender = u32 s.sender_id;
+    } <: sender_nt)
+  )
+
+val opt_tag_to_opt_bytes: option_nt mac_nt -> result (option bytes)
+let opt_tag_to_opt_bytes mac =
+  optmac <-- network_to_option mac;
+  return (
+    match optmac with
+    | None -> (None <: option bytes)
+    | Some m -> Some (m.mac_value)
+  )
+
+val opt_bytes_to_opt_tag: option bytes -> result (option_nt mac_nt)
+let opt_bytes_to_opt_tag mac =
+  optmac <-- (match mac with
+    | None -> (return None)
+    | Some m -> if Seq.length m < 256 then return (Some ({mac_value = m})) else internal_failure "opt_bytes_to_opt_tag: mac too long"
+  );
+  return (option_to_network optmac)
